Asm safety interface: progress in the proofs of memory construction

common/MemFootprint.v
@@ -156,69 +156,43 @@ Lemma inject_implies_valid_memory: forall m tm j,
     memory_valid (meminj_inv_memfp (inv_inj j m)) tm.
 Admitted.
 
+(* Move to Memory.v *)
+Lemma in_perm_nonempty: forall b o m,
+    Mem.perm m b o Max Nonempty ->
+    In o (map fst (Mem.perm_elements_any ((ZMap.elements (Mem.mem_access m) # b)))).
+Proof.
+  intros.
+  red in H. red in H. 
+  destruct (((Mem.mem_access m) # b) ## o Max) eqn: PERM; try contradiction.  
+  eapply in_map_iff. exists (o, (((Mem.mem_access m) # b) ## o)). 
+  split; auto.
+  eapply Mem.in_perm_any; eauto.
+  eapply ZMap.elements_correct; eauto.
+  rewrite Mem.access_default.
+  intro.
+  rewrite H0 in PERM. congruence.
+Qed.
 
-(** Construction of inverse injection and source memory (the same
-steps as m2'1 and m2' in Injectfootprint) *)
+(** Construction of inverse injection and source memory (m1') in the
+return *)
 
-
-Require Import Mergesort.
-
-Module ZOrder.
-  Definition t := Z.
-  Definition leb := Z.leb.
-  Lemma leb_total : forall x y : t, leb x y = true \/ leb y x = true.
-  Proof.
-    intros x y; case (Zle_bool_total x y); auto.
-  Qed.
-
-End ZOrder.
-
-Module ZSort := Mergesort.Sort(ZOrder).
-
-(* We’ll need a function to extend the current interval if the next
-element is consecutive, or start a new interval otherwise. *)
-Fixpoint intervals_aux (cur : option (Z * Z)) (l : list Z) : list (Z * Z) :=
-  match l, cur with
-  | [], None => []
-  | [], Some (a,b) => [(a,b)]
-  | x :: xs, None => intervals_aux (Some (x, Z.succ x)) xs
-  | x :: xs, Some (a,b) =>
-      if Z.eqb x b then
-        (* extend the current interval *)
-        intervals_aux (Some (a, Z.succ x)) xs
-      else
-        (* close the current interval and start a new one *)
-        (a,b) :: intervals_aux (Some (x, Z.succ x)) xs
-  end.
-
-Definition intervals (l : list Z) : list (Z*Z) :=
-  intervals_aux None l.
-
-
-Definition loc_in_reach_intervals_block (b: block) (mfp: Z -> bool) (locs: list Z) : list (block * Z * Z) :=
-  let in_reach_locs := filter mfp locs in
-  let sorted_locs := ZSort.sort in_reach_locs in
-  map (fun '(lo, hi) => (b, lo, hi)) (intervals sorted_locs).
-
-Definition loc_in_reach_intervals (s: list block) (mfp: memfp) (m: mem) : list (block * Z * Z) :=
-  concat (map (fun b => loc_in_reach_intervals_block b (mfp b)
-                       (* filter the locations that at least have Nonempty permission *)
-                       (map fst (Mem.perm_elements_any (ZMap.elements (NMap.get _ b m.(Mem.mem_access))))))
-                       s).
-
-Definition meminj_inv_add (invj: meminj_inv) (tb: block) (lo hi: Z) (sb: block) (slo: Z) : meminj_inv :=
+Definition meminj_inv_add (invj: meminj_inv) (mfp': memfp) (tb: block) (sb: block) : meminj_inv :=
   fun b ofs => 
-    if eq_block b tb && zle lo ofs && zlt ofs hi then
-      Some (sb, slo + hi - lo)
-    else
-      invj b ofs.
+    if eq_block b tb then
+      if mfp' tb ofs then 
+        Some (sb, ofs)
+      else 
+        None
+    else invj b ofs.
 
-Fixpoint update_meminj_fp' (intvs: list (block * Z * Z)) (j: meminj) (invj: meminj_inv) (s: sup) : meminj * meminj_inv * sup :=
-  match intvs with
-  | nil => (j, invj, s)
-  | (tb, lo, hi) :: tl =>
-      let sb := Mem.fresh_block s in
-      update_meminj_fp' tl (meminj_add j sb (tb, lo)) (meminj_inv_add invj tb lo hi sb 0) (sup_incr s)
+(* Given the updated footprint mfp', construct corresponded blocks for
+target blocks s2 in source memory with support s1 *)
+Fixpoint update_meminj_fp' (mfp': memfp) (s2: list block) (j: meminj) (invj: meminj_inv) (s1: sup) : meminj * meminj_inv * sup :=
+  match s2 with
+  | nil => (j, invj, s1)
+  | tb :: tl =>
+      let sb := Mem.fresh_block s1 in
+      update_meminj_fp' mfp' tl (meminj_add j sb (tb, 0)) (meminj_inv_add invj mfp' tb sb) (sup_incr s1)
   end.
 
 (* update the injection with the old injection and the new footprint,
@@ -228,9 +202,7 @@ Definition update_meminj_fp (j: meminj) (invj: meminj_inv) (m1 m2 m2': mem) (mfp
   let s2 := Mem.sup_list (Mem.support m2) in
   let s2' := Mem.sup_list (Mem.support m2') in
   let new_s2' := filter (fun b => negb (in_dec eq_block b s2)) s2' in
-  let intvs := loc_in_reach_intervals new_s2' mfp' m2' in
-  update_meminj_fp' intvs j invj (Mem.support m1).
-
+  update_meminj_fp' mfp' new_s2' j invj (Mem.support m1).
 
 (* update memory value *)
 
@@ -322,62 +294,36 @@ Definition step2_new_blocks : mem :=
 
 (* step3: copy the contents of old blocks of m1 into m1' *)
 
-(* merge two permission (choose the smaller one) *)
-
-Definition join_perm (p1 p2: permission) : permission :=
-  match p1, p2 with
-  | Nonempty, _
-  | _, Nonempty => Nonempty
-  | Readable, _
-  | _, Readable => Readable
-  | Writable, _
-  | _, Writable => Writable
-  | _, _ => Freeable
-  end.
-
-Definition join_option_perm (op1 op2: option permission) : option permission :=
-  match op1, op2 with
-  | None, _
-  | _, None => None
-  | Some p1, Some p2 => Some (join_perm p1 p2)
-  end.
-
-(* We cannot directly use the permission in the target memory as that
-in the source, because it may deviate from the permission in the old
-source memory. And also we cannot use the original permission in the
-old source memory in the new memory, as it may break the injection
-(imagine that the orignal permission is Writable, but the new target
-memory has Readable as the new permission). Therefore, we use this
-join operation to choose a righ permission. *)
-Definition join_memperm (perm1 perm2: Mem.memperm) : Mem.memperm :=
-  fun k => join_option_perm (perm1 k) (perm2 k).
-
-(* perms: the source permission *)
-Fixpoint content_perm_filter' (perms : list (Z * Mem.memperm)) (sb: block): (list (Z * memval)) * (list (Z * Mem.memperm)) :=
+(* perms: the source permission. j12 sb = Some (tb, o2) *)
+Fixpoint content_perm_filter' (perms : list (Z * Mem.memperm)) (sb tb: block) (o2: Z) : (list (Z * memval)) * (list (Z * Mem.memperm)) :=
   match perms with
   | nil => (nil, nil)
-  | (o1, p) :: tl =>
-      (* only care old injection? *)
-      match j12 sb with
-      | Some (tb, o2) =>
-          let joined_perm := join_memperm p ((Mem.mem_access m2') # tb ## (o1 + o2)%Z) in
-          let (vl, pl) := content_perm_filter' tl sb in
-          let pl' := (o1, joined_perm) :: pl in
-          (* if the original permission of this location is Readable *)
-          if Mem.perm_order'_dec (joined_perm Cur) Readable then
-            if Mem.perm_dec m1 sb o1 Max Writable then              
-              ((o1, memval_map_inv j21' ((Mem.mem_contents m2') # tb ## (o1 + o2)%Z)) :: vl,
-                pl')
-            else (vl, pl')
-          else (vl, pl')
-      (* This block is not injected *)
-      | None => content_perm_filter' tl sb 
-      end
+  | (o1, _) :: tl =>      
+      let new_perm := (Mem.mem_access m2') # tb ## (o1 + o2)%Z in
+      let (vl, pl) := content_perm_filter' tl sb tb o2 in
+      let pl' := (o1, new_perm) :: pl in
+      let m2v := (Mem.mem_contents m2') # tb ## (o1 + o2)%Z in
+      (* if the permission of this location in the target is
+          Readable (as we just copy the target permission to the
+          source, using the target permission is correct) *)
+      if Mem.perm_dec m2' tb (o1 + o2) Cur Readable then
+        if Mem.perm_dec m1 sb o1 Max Writable then 
+          ((o1, memval_map_inv j21' m2v) :: vl,
+            pl')
+        else (vl, pl')
+      else (vl, pl')
   end.
 
 Definition content_perm_filter (sb : block) :=
-  let elements := ZMap.elements ((Mem.mem_access m1) # sb) in
-  content_perm_filter' elements sb.
+  (* We use perm_elements_any because we do not want to make the
+  locations that have no permissions to be mapped locations *)
+  let elements := Mem.perm_elements_any (ZMap.elements ((Mem.mem_access m1) # sb)) in
+  match j12 sb with
+  | Some (tb, o2) => 
+      content_perm_filter' elements sb tb o2
+  | None =>
+      (nil, nil)
+  end.
 
 (* update contents and permission of all positions in vmap and
 perm_map which are from the updating memory m in inject_old_block *)
@@ -385,15 +331,178 @@ Definition copy_content_perm_old_block (sb: block) (vmap: ZMap.t memval) (perm_m
   let (vl, pl) := content_perm_filter sb in
   (Mem.setN' vl vmap, Mem.setN' pl perm_map).
 
+
+Lemma content_perm_filter_norepet: forall l sb tb o vl pl,
+    list_norepet (map fst l) ->
+    content_perm_filter' l sb tb o = (vl, pl) ->
+    list_norepet (map fst pl) /\ list_norepet (map fst vl).
+Admitted.
+
+Lemma content_perm_filter_none_aux1: forall l vl pl sb tb o1 o2,
+    ~ In o1 (map fst l) ->
+    content_perm_filter' l sb tb o2 = (vl, pl) ->
+    ~ In o1 (map fst vl).
+Proof.
+  induction l; intros. simpl in H0. inv H0. auto.
+  simpl in H. eapply Decidable.not_or in H.
+  destruct a as (o1' & p). simpl in H.
+  destruct H as (A & B).
+  simpl in H0.
+  destruct content_perm_filter' as (vl1 & pl1) eqn: F in H0.
+  destruct (Mem.perm_dec m2' tb (o1' + o2) Cur Readable).
+    + destruct (Mem.perm_dec m1 sb o1' Max Writable); inv H0; simpl.
+      * intro. destruct H; eauto.
+        eapply IHl; eauto.
+      * eauto.
+    + inv H0. eauto.
+Qed.
+
+Lemma content_perm_filter_none_aux2: forall l vl pl sb tb o1 o2 (NOREP: list_norepet (map fst l)),
+    In o1 (map fst l) ->
+    content_perm_filter' l sb tb o2 = (vl, pl) ->
+    (~ Mem.perm m2' tb (o1 + o2) Cur Readable \/
+       ~ Mem.perm m1 sb o1 Max Writable) ->
+    ~ In o1 (map fst vl).
+Proof.
+  induction l; intros. inv H.
+  inv H.
+  - simpl in H0. destruct a as (o1 & p).
+    inv NOREP.
+    destruct content_perm_filter' as (vl1 & pl1) eqn: F in H0.
+    simpl in H1. destruct H1.
+    + destruct (Mem.perm_dec m2' tb (o1 + o2) Cur Readable); try congruence.
+      inv H0. simpl. eapply content_perm_filter_none_aux1; eauto.
+    + destruct (Mem.perm_dec m2' tb (o1 + o2) Cur Readable).
+      * destruct (Mem.perm_dec m1 sb o1 Max Writable); try congruence.
+        inv H0. simpl. eapply content_perm_filter_none_aux1; eauto.
+      * inv H0. simpl. eapply content_perm_filter_none_aux1; eauto.
+  - inv NOREP. simpl in H0.
+    destruct a as (o1' & p).
+    destruct content_perm_filter' as (vl1 & pl1) eqn: F in H0.
+    destruct (Mem.perm_dec m2' tb (o1' + o2) Cur Readable).
+    + destruct (Mem.perm_dec m1 sb o1' Max Writable); inv H0.
+      * simpl. intro. destruct H.
+        -- subst. simpl in H4. congruence.
+        -- eapply IHl; eauto.
+      * eapply IHl; eauto.
+    + inv H0. eapply IHl; eauto.
+Qed.
+
+Lemma content_perm_filter_none: forall vl pl sb tb o1 o2,
+    content_perm_filter' (Mem.perm_elements_any (ZMap.elements (Mem.mem_access m1) # sb)) sb tb o2 = (vl, pl) ->
+    Mem.perm m1 sb o1 Max Nonempty ->
+    (~ Mem.perm m2' tb (o1 + o2) Cur Readable \/
+       ~ Mem.perm m1 sb o1 Max Writable) ->
+    ~ In o1 (map fst vl).
+Proof.
+  intros. eapply content_perm_filter_none_aux2; eauto.
+  eapply Mem.fst_perm_any_norepet. eapply ZMap.elements_keys_norepet.
+  eapply in_perm_nonempty. auto.
+Qed.
+
+Lemma content_perm_filter_some_aux: forall l vl pl sb tb o1 o2,
+    In o1 (map fst l) ->
+    content_perm_filter' l sb tb o2 = (vl, pl) ->
+    In (o1, ((Mem.mem_access m2') # tb) ## (o1 + o2)) pl
+    /\ (Mem.perm m2' tb (o1 + o2) Cur Readable ->            
+       Mem.perm m1 sb o1 Max Writable ->
+       In (o1, memval_map_inv j21' ((Mem.mem_contents m2') # tb) ## (o1 + o2)) vl).
+Proof.
+  induction l; intros. inv H.
+  inv H. 
+  - simpl in H0. destruct a as (o1 & p).
+    destruct content_perm_filter' as (vl1 & pl1) in H0.
+    destruct (Mem.perm_dec m2' tb (o1 + o2) Cur Readable).
+    + destruct (Mem.perm_dec m1 sb o1 Max Writable).
+      * inv H0. simpl. split; auto.
+      * inv H0. simpl. split; auto.
+        intros. contradiction.
+    + inv H0. simpl. split; auto.
+      intros. contradiction.
+  - simpl in H0.
+    destruct a as (o1' & p).
+    destruct content_perm_filter' as (vl1 & pl1) eqn: F in H0.
+    destruct (Mem.perm_dec m2' tb (o1' + o2) Cur Readable).
+    + destruct (Mem.perm_dec m1 sb o1' Max Writable).
+      * inv H0. simpl. split; auto.
+        right.
+        eapply IHl; eauto.
+        intros. right.
+        eapply IHl; eauto.
+      * inv H0. simpl. split; auto.
+        right.
+        eapply IHl; eauto.
+        intros. eapply IHl; eauto.
+    + inv H0. simpl. split; auto.
+      right.
+      eapply IHl; eauto.
+      intros. eapply IHl; eauto.
+Qed.
+
+Lemma content_perm_filter_some: forall vl pl sb tb o1 o2,
+    content_perm_filter' (Mem.perm_elements_any (ZMap.elements (Mem.mem_access m1) # sb)) sb tb o2 = (vl, pl) ->
+    Mem.perm m1 sb o1 Max Nonempty ->
+    In (o1, ((Mem.mem_access m2') # tb) ## (o1 + o2)) pl
+    /\ (Mem.perm m2' tb (o1 + o2) Cur Readable ->            
+       Mem.perm m1 sb o1 Max Writable ->
+       In (o1, memval_map_inv j21' ((Mem.mem_contents m2') # tb) ## (o1 + o2)) vl).
+Proof.
+  intros. 
+  eapply content_perm_filter_some_aux; eauto.
+  eapply in_perm_nonempty. auto.
+Qed.
+
+Lemma copy_content_perm_old_block_result: forall sb vmap perm_map vmap' perm_map' o1,
+    copy_content_perm_old_block sb vmap perm_map = (vmap', perm_map') ->
+    Mem.perm m1 sb o1 Max Nonempty ->
+    vmap' ## o1 = match j12 sb with
+                   | Some (tb, o2) => 
+                       let new_perm := (Mem.mem_access m2') # tb ## (o1 + o2)%Z in
+                       let m2v := ((Mem.mem_contents m2')#tb)## (o1 + o2)%Z in
+                       if Mem.perm_dec m2' tb (o1 + o2) Cur Readable then
+                         if Mem.perm_dec m1 sb o1 Max Writable then              
+                           memval_map_inv j21' m2v 
+                         else vmap ## o1 else vmap ## o1
+                  | None => vmap## o1
+                  end
+    /\ perm_map' ## o1 = match j12 sb with
+                        | Some (tb, o2) => 
+                            (Mem.mem_access m2') # tb ## (o1 + o2)
+                        | None => 
+                            perm_map ## o1
+                        end.
+Proof.
+  intros until o1. intros COPY PERM.
+  unfold copy_content_perm_old_block, content_perm_filter in COPY.
+  destruct (j12 sb) as [ [tb o2]|] eqn: INJSB.
+  - simpl. 
+    destruct content_perm_filter' as (vl & pl) eqn: F. inv COPY.
+    exploit content_perm_filter_norepet; eauto.
+    eapply Mem.fst_perm_any_norepet.
+    eapply ZMap.elements_keys_norepet. intros (N1 & N2).
+    exploit content_perm_filter_some; eauto.
+    intros (A1 & A2).
+    destruct (Mem.perm_dec m2' tb (o1 + o2) Cur Readable).
+    + destruct (Mem.perm_dec m1 sb o1 Max Writable).
+      * erewrite !Mem.setN'_inside; eauto. 
+      * erewrite Mem.setN'_outside. 
+        erewrite !Mem.setN'_inside; eauto.
+        eapply content_perm_filter_none; eauto.
+    + erewrite Mem.setN'_outside. 
+      erewrite !Mem.setN'_inside; eauto.
+      eapply content_perm_filter_none; eauto.
+  - simpl in COPY. inv COPY. split; reflexivity.
+Qed.
+
 Program Definition inject_old_block (m: mem) (sb: block) := 
-  if j12' sb then
-    if Mem.sup_dec sb (Mem.support m) then
-      let (vm, pm) := copy_content_perm_old_block sb ((Mem.mem_contents m) # sb) ((Mem.mem_access m) # sb) in
-      {| Mem.mem_contents := NMap.set _ sb vm (Mem.mem_contents m);
-        Mem.mem_access := NMap.set _ sb pm (Mem.mem_access m);
-        Mem.support := Mem.support m |}
-    else m
+  (* if j12' sb then *)
+  if Mem.sup_dec sb (Mem.support m) then
+    let (vm, pm) := copy_content_perm_old_block sb ((Mem.mem_contents m) # sb) ((Mem.mem_access m) # sb) in
+  {| Mem.mem_contents := NMap.set _ sb vm (Mem.mem_contents m);
+    Mem.mem_access := NMap.set _ sb pm (Mem.mem_access m);
+    Mem.support := Mem.support m |}
   else m.
+  (* else m. *)
 Next Obligation. Admitted.
 Next Obligation. Admitted.
 Next Obligation. Admitted.
@@ -404,6 +513,15 @@ Fixpoint copy_old_sup' (bl:list block) m : mem :=
    | nil => m
    | hd :: tl => inject_old_block (copy_old_sup' tl m) hd
    end.
+
+ Lemma copy_old_sup'_support : forall s m,
+ Mem.support (copy_old_sup' s m) = Mem.support m.
+ Proof.
+   induction s; intros; simpl; auto.
+   unfold inject_old_block. destruct Mem.sup_dec; simpl; auto.
+   destruct copy_content_perm_old_block.
+   simpl. auto.
+ Qed.
 
 (* Copy the contents and permissions in (support m1) into m1' *)
 Definition step3_old_blocks (s: sup) m : mem := copy_old_sup' (Mem.sup_list s) m.
@@ -429,12 +547,11 @@ Section CONSTR_PROOF.
   Hypothesis INCRDISJ1 : inject_incr_disjoint j12 j12' (Mem.support m1) (Mem.support m2).
   Hypothesis INCRNOLAP'1:inject_incr_no_overlap' j12 j12'.
   (* Hypothesis MAXPERM1 : injp_max_perm_decrease m1 m1'. *)
-  (* Hypothesis IMGIN1': inject_image_in j12' s2'. *)
+  Hypothesis IMGIN1': inject_image_in j12' (Mem.support m2').
   (* Hypothesis DOMIN2': inject_dom_in j2' s2'. *)
   Hypothesis DOMIN1': inject_dom_in j12' s1'.
-  (* Hypothesis INCRNEW1: inject_incr_newblock1 j12 j1' (Mem.support m2). *)
-  (* Hypothesis INCRNEW2: inject_incr_newblock2 j2 j2' (Mem.support m2). *)
-  (* Hypothesis ADDZERO: update_add_zero j1 j1'. *)
+  Hypothesis INCRNEW1: inject_incr_newblock1 j12 j12' (Mem.support m2).
+  Hypothesis ADDZERO: update_add_zero j12 j12'.
   (* Hypothesis ADDEXISTS: update_add_exists j1 j1' (compose_meminj j1' j2'). *)
   (* Hypothesis ADDSAME : update_add_same j2 j2' j1'. *)
   (* Hypothesis ADDBLOCK: update_add_block (Mem.support m2) s2' j1' j2'. *)
@@ -442,13 +559,96 @@ Section CONSTR_PROOF.
   Definition m1'1 := step2_new_blocks m1 m2 m2' s1' j12 j12' j21' SUPINCR1.
   Definition m1' := step3_old_blocks m1 m2 m2' s1' j12 j12' j21' SUPINCR1 (Mem.support m1) m1'1.
   
+  Lemma m1'1_support : Mem.support m1'1 = s1'.
+  Proof. unfold m1'1. Admitted.
+  Lemma m1'_support : Mem.support m1' = s1'.
+  Proof. Admitted.
+
+  Lemma step3_old_blocks_sup_perm1: forall m b1 o1 b2 o2 k p,
+        j12 b1 = Some (b2, o2 - o1) ->
+        Mem.perm m1 b1 o1 Max Nonempty ->
+        Mem.support m = s1' ->
+        Mem.perm (inject_old_block m1 m2 m2' s1' j12 j12' j21' SUPINCR1 m b1) b1 o1 k p <-> Mem.perm m2' b2 o2 k p.
+  Proof.
+    intros. unfold inject_old_block.
+    exploit DOMIN1. eauto. intros SUP1. 
+    assert (SUP1' : sup_In b1 (Mem.support m)).
+    { eapply SUPINCR1 in SUP1. rewrite H1. auto. }
+    destruct Mem.sup_dec; try congruence.
+    unfold copy_content_perm_old_block. 
+    destruct (content_perm_filter m1 m2' j12 j21' b1) as (vl & pl) eqn: F.
+    unfold Mem.perm. simpl. 
+    setoid_rewrite NMap.gss.
+    exploit (copy_content_perm_old_block_result m1 m2 m2' s1' j12 j12' j21' SUPINCR1 b1 ((Mem.mem_contents m) # b1) ((Mem.mem_access m) # b1)).
+    unfold copy_content_perm_old_block. rewrite F. reflexivity.
+    instantiate (1 := o1). auto. rewrite H. simpl.
+    intros (A & B).
+    rewrite B. replace (o1 + (o2 - o1)) with o2 by lia. reflexivity.
+  Qed.
+  
+  Lemma step3_old_blocks_sup_perm2: forall m b b1 o1 k p,
+      b <> b1 ->
+      Mem.perm (inject_old_block m1 m2 m2' s1' j12 j12' j21' SUPINCR1 m b) b1 o1 k p <-> Mem.perm m b1 o1 k p.
+  Proof.
+    intros. unfold inject_old_block.
+    destruct Mem.sup_dec.
+    - destruct copy_content_perm_old_block.
+      unfold Mem.perm. simpl.
+      setoid_rewrite NMap.gso; try congruence.
+      reflexivity.
+    - reflexivity.
+  Qed.      
+    
+  Lemma step3_old_blocks_sup_perm: forall bl m b1 o1 b2 o2 k p,
+        j12 b1 = Some (b2, o2 - o1) ->
+        Mem.perm m1 b1 o1 Max Nonempty ->
+        In b1 bl ->
+        Mem.support m = s1' ->
+        Mem.perm (copy_old_sup' m1 m2 m2' s1' j12 j12' j21' SUPINCR1 bl m) b1 o1 k p <-> Mem.perm m2' b2 o2 k p.
+  Proof.
+    induction bl; intros.
+    - inv H1.
+    - simpl. destruct (eq_block b1 a).
+      + subst a. 
+        eapply step3_old_blocks_sup_perm1; eauto.
+        rewrite <- H2. eapply copy_old_sup'_support.
+      + destruct H1. congruence.
+        etransitivity.
+        eapply step3_old_blocks_sup_perm2; eauto.
+        eauto.
+  Qed.
+
   Lemma old_injected_block_perm: forall b1 o1 b2 o2 k p,
+          j12 b1 = Some (b2, o2 - o1) ->
+          Mem.perm m1 b1 o1 Max Nonempty ->
+          Mem.perm m1' b1 o1 k p <->
+          Mem.perm m2' b2 o2 k p.
+  Proof.
+    intros. unfold m1'.
+    eapply step3_old_blocks_sup_perm; eauto.
+    eapply DOMIN1. eauto.
+    eapply m1'1_support.
+  Qed.
+
+  Lemma old_injected_block_perm1: forall b1 o1 b2 o2 k p,
           j12 b1 = Some (b2, o2 - o1) ->
           Mem.perm m1 b1 o1 Max Nonempty ->
           Mem.perm m1' b1 o1 k p ->
           Mem.perm m2' b2 o2 k p.
   Proof.
-  Admitted.
+    intros. eapply old_injected_block_perm; eauto.
+  Qed.
+
+
+  Lemma old_injected_block_perm2: forall b1 o1 b2 o2 k p,
+          j12 b1 = Some (b2, o2 - o1) ->
+          Mem.perm m1 b1 o1 Max Nonempty ->
+          Mem.perm m2' b2 o2 k p ->
+          Mem.perm m1' b1 o1 k p.
+  Proof.
+    intros. eapply old_injected_block_perm; eauto.
+  Qed.
+
 
   Lemma new_injected_block_perm: forall b1 o1 b2 o2 k p,
       j12 b1 = None ->      
@@ -463,20 +663,41 @@ Section CONSTR_PROOF.
   Lemma new_injected_block_perm1: forall b1 o1 b2 o2 k p,
       j12 b1 = None ->      
       j12' b1 = Some (b2, o2 - o1) ->
-      Mem.perm m1' b1 o1 Max Nonempty ->
-      (Mem.perm m1' b1 o1 k p ->
-         Mem.perm m2' b2 o2 k p).
+      Mem.perm m1' b1 o1 k p ->
+      Mem.perm m2' b2 o2 k p.
   Proof.
     intros. eapply new_injected_block_perm; eauto.
+    eauto with mem.
   Qed.
-  
+
   Lemma new_injected_block_perm2: forall b1 o1 b2 o2 k p,
       j12 b1 = None ->      
       j12' b1 = Some (b2, o2 - o1) ->
+      Mem.perm m1' b1 o1 Max Nonempty ->      
       Mem.perm m2' b2 o2 k p ->
       Mem.perm m1' b1 o1 k p.
   Proof.
-    (* prove that m1'[(b1,o1)] is Nonempty *)
+    intros.
+    eapply new_injected_block_perm; eauto.
+  Qed.
+
+
+  (* similar to copy_content_inject *)
+  Lemma old_injected_block_content_inject : forall b1 o1 b2 o2,
+      j12 b1 = Some (b2, o2 - o1) ->
+      Mem.perm m1' b1 o1 Cur Readable ->
+      Mem.perm m1 b1 o1 Max Writable ->
+      memval_inject j12' (mem_memval m1' b1 o1) (mem_memval m2' b2 o2).
+  Proof.
+  Admitted.
+
+  (* similar to step2_content_inject *)
+  Lemma new_injected_block_content_inject : forall b1 o1 b2 o2,
+      j12 b1 = None ->
+      j12' b1 = Some (b2, o2 - o1) ->
+      Mem.perm m1' b1 o1 Cur Readable ->     
+      memval_inject j12' (mem_memval m1' b1 o1) (mem_memval m2' b2 o2).
+  Proof.
   Admitted.
 
 
@@ -490,6 +711,8 @@ Section CONSTR_PROOF.
   Lemma UNC2: Mem.unchanged_on (loc_out_of_reach j12 m1) m2 m2'.
   Admitted.
 
+  Lemma ROUNC1: Mem.ro_unchanged m1 m1'.
+  Admitted.
 
   Lemma INJ12': Mem.inject j12' m1' m2'.
   Proof.
@@ -508,20 +731,75 @@ Section CONSTR_PROOF.
         (* new injected block *)
         * eapply new_injected_block_perm1 with (o1 := ofs); eauto.
           replace (ofs + delta - ofs) with delta by lia. auto.
-          eauto with mem.
       (* alignment *)
       + intros.
         destruct (subinj_dec j12 j12' b1 b2 delta INCR1 H).
         * eapply Mem.mi_align. eapply INJ12. eauto.
           red. intros. eapply MAXPERM1. eapply DOMIN1. eauto.
           eapply H0. eauto.
-        * Mem.inject'
-memory_valid align_chunk
-                         Mem.inject'
-        
-
-  Lemma ROUNC1: Mem.ro_unchanged m1 m1'.
-  Admitted.
+        * exploit ADDZERO; eauto. intros. subst.
+          eapply Z.divide_0_r.
+      (* contents *)
+      + intros.
+        destruct (subinj_dec j12 j12' b1 b2 delta INCR1 H).
+        * destruct (Mem.perm_dec m1 b1 ofs Max Writable).
+          -- eapply old_injected_block_content_inject; eauto.
+             replace (ofs + delta - ofs) with delta by lia. eauto. 
+          (* The location is not Writable in m1 *)
+          -- generalize ROUNC1. intros ROUNC1.
+             apply Mem.ro_unchanged_memval_bytes in ROUNC2 as ROUNC2'.
+             apply Mem.ro_unchanged_memval_bytes in ROUNC1 as ROUNC1'.
+             exploit ROUNC1'; eauto. 
+             eapply Mem.valid_block_inject_1; eauto.
+             intros [PERM1 MVAL1]. rewrite <- MVAL1.
+             assert (NOTWRITE: ~ Mem.perm m2 b2 (ofs + delta) Max Writable).
+             { intro. exploit Mem.mi_perm_inv; eauto. intros [A|B].
+               - congruence.
+               - eapply B. eauto with mem. }             
+             exploit ROUNC2'; eauto.
+             eapply Mem.valid_block_inject_2. apply e. eauto.
+             eapply old_injected_block_perm; eauto.
+             replace (ofs + delta - ofs) with delta by lia. auto.
+             eauto with mem.
+             intros [PERM2 MVAL2]. rewrite <- MVAL2.
+             inversion INJ12. inversion mi_inj.
+             eapply memval_inject_incr; eauto.
+        (* new injected block *)
+        * eapply new_injected_block_content_inject; eauto.
+          replace (ofs + delta - ofs) with delta by lia. auto.
+    (* mi_freeblocks *)
+    - intros.
+      destruct (j12' b) as [[b2 d]|] eqn:?; auto.
+      eapply DOMIN1' in Heqo. rewrite <- m1'_support in Heqo.
+      exfalso. eapply H. eauto.
+    (* mi_mappedblocks *)
+    - intros. red. eapply IMGIN1'. eauto.
+    - eapply update_meminj_no_overlap1. eapply MAXPERM1.
+      all: eauto. 
+    (* mi_representable *)
+    - intros. destruct (j12 b) as [[b2' d']|] eqn: Hj1b.
+      + apply INCR1 in Hj1b as H'. rewrite H in H'. inv H'.
+        inversion INJ12.
+        eapply mi_representable; eauto.
+        destruct H0.
+        left. eapply MAXPERM1; eauto. unfold Mem.valid_block. eauto.
+        right. eapply MAXPERM1; eauto. unfold Mem.valid_block. eauto.
+      + exploit ADDZERO; eauto. intro. subst. split. lia.
+        generalize (Ptrofs.unsigned_range_2 ofs). lia.
+    (* mi_perm_inv *)
+    - intros. 
+      destruct (subinj_dec j12 j12' b1 b2 delta INCR1 H).
+      + destruct (Mem.perm_dec m1' b1 ofs Max Nonempty); eauto.
+        left.
+        eapply old_injected_block_perm2; eauto.
+        replace (ofs + delta - ofs) with delta by lia. auto.
+        eapply MAXPERM1; eauto.
+        eapply DOMIN1. eauto.
+      + destruct (Mem.perm_dec m1' b1 ofs Max Nonempty); eauto.
+        left.
+        eapply new_injected_block_perm2; eauto.
+        replace (ofs + delta - ofs) with delta by lia. auto.
+Qed.
 
 
 End CONSTR_PROOF.
